Some updates on soundness (#132)
* Update some soundness/algorithmic parts

* Add some notations for gluing

* Add some more to soundness

* Make glu model unary

* Some changes

* Add some more

theories/Core/Soundness/LogicalRelation/Definitions.v
@@ -10,281 +10,358 @@ Global Open Scope predicate_scope.
 
 Generalizable All Variables.
 
-Notation "'typ_pred'" := (predicate (Tcons ctx (Tcons typ Tnil))).
-Notation "'typ_pred_equivalence'" := (@predicate_equivalence (Tcons ctx (Tcons typ Tnil))).
-Notation "'glu_pred'" := (predicate (Tcons ctx (Tcons exp (Tcons typ (Tcons domain Tnil))))).
-Notation "'glu_pred_equivalence'" := (@predicate_equivalence (Tcons ctx (Tcons exp (Tcons typ (Tcons domain Tnil))))).
+Notation "'glu_typ_pred_args'" := (Tcons ctx (Tcons typ Tnil)).
+Notation "'glu_typ_pred'" := (predicate glu_typ_pred_args).
+Notation "'glu_typ_pred_equivalence'" := (@predicate_equivalence glu_typ_pred_args).
+Notation "Γ ⊢ A ® R" := ((R Γ A : Prop) : Prop) (in custom judg at level 80, Γ custom exp, A custom exp, R constr).
 
-Definition univ_typ_pred j i : typ_pred := fun Γ T => {{ Γ ⊢ T ≈ Type@j :  Type@i }}.
-Arguments univ_typ_pred j i Γ T/.
+Notation "'glu_exp_pred_args'" := (Tcons ctx (Tcons exp (Tcons typ (Tcons domain Tnil)))).
+Notation "'glu_exp_pred'" := (predicate glu_exp_pred_args).
+Notation "'glu_exp_pred_equivalence'" := (@predicate_equivalence glu_exp_pred_args).
+Notation "Γ ⊢ M : A ® m ∈ R" := (R Γ M A m : (Prop : Type)) (in custom judg at level 80, Γ custom exp, M custom exp, A custom exp, m custom domain, R constr).
+
+Notation "'glu_sub_pred_args'" := (Tcons ctx (Tcons sub (Tcons env Tnil))).
+Notation "'glu_sub_pred'" := (predicate glu_sub_pred_args).
+Notation "'glu_sub_pred_equivalence'" := (@predicate_equivalence glu_sub_pred_args).
+Notation "Γ ⊢s σ ® ρ ∈ R" := (R Γ σ ρ : Prop) (in custom judg at level 80, Γ custom exp, σ custom exp, ρ custom domain, R constr).
+
+Notation "'DG' a ∈ R ↘ P ↘ El" := (R P El a : Prop) (in custom judg at level 90, a custom domain, R constr, P constr, El constr).
+Notation "'EG' A ∈ R ↘ Sb " := (R Sb A : Prop) (in custom judg at level 90, A custom exp, R constr, Sb constr).
 
 Inductive glu_nat : ctx -> exp -> domain -> Prop :=
 | glu_nat_zero :
-  `( {{ Γ ⊢ m ≈ zero : ℕ }} ->
-     glu_nat Γ m d{{{ zero }}} )
+  `{ {{ Γ ⊢ m ≈ zero : ℕ }} ->
+     glu_nat Γ m d{{{ zero }}} }
 | glu_nat_succ :
-  `( {{ Γ ⊢ m ≈ succ m' : ℕ }} ->
+  `{ {{ Γ ⊢ m ≈ succ m' : ℕ }} ->
      glu_nat Γ m' a ->
-     glu_nat Γ m d{{{ succ a }}} )
+     glu_nat Γ m d{{{ succ a }}} }
 | glu_nat_neut :
-  `( per_bot c c ->
-     (forall {Δ σ v}, {{ Δ ⊢w σ : Γ }} -> {{ Rne c in length Δ ↘ v }} -> {{ Δ ⊢ m [ σ ] ≈ v : ℕ }}) ->
-     glu_nat Γ m d{{{ ⇑ ℕ c }}} ).
+  `{ per_bot c c ->
+     (forall {Δ σ v}, {{ Δ ⊢w σ : Γ }} -> {{ Rne c in length Δ ↘ v }} -> {{ Δ ⊢ m[σ] ≈ v : ℕ }}) ->
+     glu_nat Γ m d{{{ ⇑ ℕ c }}} }.
 
 #[export]
- Hint Constructors glu_nat : mcltt.
+Hint Constructors glu_nat : mcltt.
 
-Definition nat_typ_pred i : typ_pred := fun Γ M => {{ Γ ⊢ M ≈ ℕ : Type@i }}.
-Arguments nat_typ_pred i Γ M/.
+Definition nat_glu_typ_pred i : glu_typ_pred := fun Γ M => {{ Γ ⊢ M ≈ ℕ : Type@i }}.
+Arguments nat_glu_typ_pred i Γ M/.
 
-Definition nat_glu_pred i : glu_pred := fun Γ m M a => nat_typ_pred i Γ M /\ glu_nat Γ m a.
-Arguments nat_glu_pred i Γ m M a/.
+Definition nat_glu_exp_pred i : glu_exp_pred := fun Γ m M a => {{ Γ ⊢ M ® nat_glu_typ_pred i }} /\ glu_nat Γ m a.
+Arguments nat_glu_exp_pred i Γ m M a/.
 
-Definition neut_typ_pred i C : typ_pred :=
+Definition neut_glu_typ_pred i C : glu_typ_pred :=
   fun Γ M => {{ Γ ⊢ M : Type@i }} /\
-            (forall Δ σ V, {{ Δ ⊢w σ : Γ }} -> {{ Rne C in length Δ ↘ V }} -> {{ Δ ⊢ M [ σ ] ≈ V : Type@i }}).
-Arguments neut_typ_pred i C Γ M/.
+            (forall Δ σ V, {{ Δ ⊢w σ : Γ }} -> {{ Rne C in length Δ ↘ V }} -> {{ Δ ⊢ M[σ] ≈ V : Type@i }}).
+Arguments neut_glu_typ_pred i C Γ M/.
 
-Inductive neut_glu_pred i C : glu_pred :=
-| ngp_make : forall Γ m M A c,
-    neut_typ_pred i C Γ M ->
-    per_bot c c ->
-    (forall Δ σ V v, {{ Δ ⊢w σ : Γ }} ->
-                {{ Rne C in length Δ ↘ V }} ->
-                {{ Rne c in length Δ ↘ v }} ->
-                {{ Δ ⊢ m [ σ ] ≈ v : M [ σ ] }}) ->
-    neut_glu_pred i C Γ m M d{{{ ⇑ A c }}}.
+Inductive neut_glu_exp_pred i C : glu_exp_pred :=
+| mk_neut_glu_exp_pred :
+    `{ {{ Γ ⊢ M ® neut_glu_typ_pred i C }} ->
+       {{ Dom c ≈ c ∈ per_bot }} ->
+       (forall Δ σ V v, {{ Δ ⊢w σ : Γ }} ->
+                      {{ Rne C in length Δ ↘ V }} ->
+                      {{ Rne c in length Δ ↘ v }} ->
+                      {{ Δ ⊢ m[σ] ≈ v : M[σ] }}) ->
+       {{ Γ ⊢ m : M ® ⇑ A c ∈ neut_glu_exp_pred i C }} }.
 
-Inductive pi_typ_pred i
+Inductive pi_glu_typ_pred i
   (IR : relation domain)
-  (IP : typ_pred)
-  (IEl : glu_pred)
-  (OP : forall c c' (equiv_c_c' : {{ Dom c ≈ c' ∈ IR }}),  typ_pred) : typ_pred :=
-| ptp_make : forall Γ IT OT M,
-    {{ Γ ⊢ M ≈ Π IT OT : Type@i }} ->
-    {{ Γ , IT ⊢ OT : Type@i }} ->
-    (forall Δ σ, {{ Δ ⊢w σ : Γ }} -> IP Δ {{{ IT [ σ ] }}}) ->
-    (forall Δ σ m a, {{ Δ ⊢w σ : Γ }} -> IEl Δ m {{{ IT [ σ ] }}} a -> forall (Ha : IR a a), OP _ _ Ha Δ {{{ OT [ σ ,, m ] }}}) ->
-    pi_typ_pred i IR IP IEl OP Γ M.
+  (IP : glu_typ_pred)
+  (IEl : glu_exp_pred)
+  (OP : forall c (equiv_c : {{ Dom c ≈ c ∈ IR }}), glu_typ_pred) : glu_typ_pred :=
+| mk_pi_glu_typ_pred :
+    `{ {{ Γ ⊢ M ≈ Π IT OT : Type@i }} ->
+       {{ Γ , IT ⊢ OT : Type@i }} ->
+       (forall Δ σ, {{ Δ ⊢w σ : Γ }} -> {{ Δ ⊢ IT[σ] ® IP }}) ->
+       (forall Δ σ m a,
+           {{ Δ ⊢w σ : Γ }} ->
+           {{ Δ ⊢ m : IT[σ] ® a ∈ IEl }} ->
+           forall (equiv_a_a : {{ Dom a ≈ a ∈ IR }}),
+             {{ Δ ⊢ OT[σ,,m] ® OP _ equiv_a_a }}) ->
+       {{ Γ ⊢ M ® pi_glu_typ_pred i IR IP IEl OP }} }.
 
-Inductive pi_glu_pred i
+Inductive pi_glu_exp_pred i
   (IR : relation domain)
-  (IP : typ_pred)
-  (IEl : glu_pred)
+  (IP : glu_typ_pred)
+  (IEl : glu_exp_pred)
   (elem_rel : relation domain)
-  (OEl : forall c c' (equiv_c_c' : {{ Dom c ≈ c' ∈ IR }}),  glu_pred): glu_pred :=
-| pgp_make : forall Γ IT OT m M a,
-    {{ Γ ⊢ m : M }} ->
-    elem_rel a a ->
-    {{ Γ ⊢ M ≈ Π IT OT : Type@i }} ->
-    {{ Γ , IT ⊢ OT : Type@i }} ->
-    (forall Δ σ, {{ Δ ⊢w σ : Γ }} -> IP Δ {{{ IT [ σ ] }}}) ->
-    (forall Δ σ m' b, {{ Δ ⊢w σ : Γ }} -> IEl Δ m' {{{ IT [ σ ] }}} b -> forall (Ha : IR b b),
-                   exists ab, {{ $| a & b |↘ ab }} /\ OEl _ _ Ha Δ {{{ m [ σ ] m' }}} {{{ OT [ σ ,, m' ] }}} ab) ->
-    pi_glu_pred i IR IP IEl elem_rel OEl Γ m M a.
+  (OEl : forall c (equiv_c : {{ Dom c ≈ c ∈ IR }}), glu_exp_pred): glu_exp_pred :=
+| mk_pi_glu_exp_pred :
+  `{ {{ Γ ⊢ m : M }} ->
+     {{ Dom a ≈ a ∈ elem_rel }} ->
+     {{ Γ ⊢ M ≈ Π IT OT : Type@i }} ->
+     {{ Γ , IT ⊢ OT : Type@i }} ->
+     (forall Δ σ, {{ Δ ⊢w σ : Γ }} -> {{ Δ ⊢ IT[σ] ® IP }}) ->
+     (forall Δ σ m' b,
+         {{ Δ ⊢w σ : Γ }} ->
+         {{ Δ ⊢ m' : IT[ σ ] ® b ∈ IEl }} ->
+         forall (equiv_b_b : {{ Dom b ≈ b ∈ IR }}),
+         exists ab, {{ $| a & b |↘ ab }} /\ {{ Δ ⊢ m[σ] m' : OT[σ,,m'] ® ab ∈ OEl _ equiv_b_b }}) ->
+     {{ Γ ⊢ m : M ® a ∈ pi_glu_exp_pred i IR IP IEl elem_rel OEl }} }.
 
 #[export]
- Hint Constructors neut_glu_pred pi_typ_pred pi_glu_pred : mcltt.
+Hint Constructors neut_glu_exp_pred pi_glu_typ_pred pi_glu_exp_pred : mcltt.
 
-Lemma pi_glu_pred_pi_typ_pred : forall i IR IP IEl (OP : forall c c' (equiv_c_c' : {{ Dom c ≈ c' ∈ IR }}),  typ_pred) elem_rel OEl Γ m M a,
-    pi_glu_pred i IR IP IEl elem_rel OEl Γ m M a ->
-    (forall Δ m' M' b c c' (Hc : IR c c'), OEl _ _ Hc Δ m' M' b -> OP _ _ Hc Δ M') ->
-    pi_typ_pred i IR IP IEl OP Γ M.
-Proof.
-  inversion_clear 1; econstructor; eauto.
-  intros.
-  edestruct H5 as [? []]; eauto.
-Qed.
+Definition univ_glu_typ_pred j i : glu_typ_pred := fun Γ T => {{ Γ ⊢ T ≈ Type@j :  Type@i }}.
+Arguments univ_glu_typ_pred j i Γ T/.
 
 Section Gluing.
   Variable
     (i : nat)
-      (glu_univ_typ_rec : forall {j}, j < i -> domain -> typ_pred).
+      (glu_univ_typ_rec : forall {j}, j < i -> domain -> glu_typ_pred).
 
-  Definition univ_glu_pred' {j} (lt_j_i : j < i) : glu_pred :=
+  Definition univ_glu_exp_pred' {j} (lt_j_i : j < i) : glu_exp_pred :=
     fun Γ m M A =>
-      {{ Γ ⊢ m : M }} /\ {{ Γ ⊢ M ≈ Type@j : Type@i }} /\
-        per_univ j A A /\
-        glu_univ_typ_rec lt_j_i A Γ m.
+      {{ Γ ⊢ m : M }} /\
+        {{ Γ ⊢ M ≈ Type@j : Type@i }} /\
+        {{ Γ ⊢ m ® glu_univ_typ_rec lt_j_i A }}.
 
   #[global]
-    Arguments univ_glu_pred' {j} lt_j_i Γ m M A/.
+  Arguments univ_glu_exp_pred' {j} lt_j_i Γ m M A/.
 
-  Inductive glu_univ_elem_core : typ_pred -> glu_pred -> domain -> domain -> Prop :=
+  Inductive glu_univ_elem_core : glu_typ_pred -> glu_exp_pred -> domain -> Prop :=
   | glu_univ_elem_core_univ :
     `{ forall typ_rel
          el_rel
          (lt_j_i : j < i),
-          j = j' ->
-          typ_rel <∙> univ_typ_pred j i ->
-          el_rel <∙> univ_glu_pred' lt_j_i ->
-          glu_univ_elem_core typ_rel el_rel d{{{ 𝕌@j }}} d{{{ 𝕌@j' }}} }
+          typ_rel <∙> univ_glu_typ_pred j i ->
+          el_rel <∙> univ_glu_exp_pred' lt_j_i ->
+          {{ DG 𝕌@j ∈ glu_univ_elem_core ↘ typ_rel ↘ el_rel }} }
 
   | glu_univ_elem_core_nat :
     `{ forall typ_rel el_rel,
-          typ_rel <∙> nat_typ_pred i ->
-          el_rel <∙> nat_glu_pred i ->
-          glu_univ_elem_core typ_rel el_rel d{{{ ℕ }}} d{{{ ℕ }}} }
+          typ_rel <∙> nat_glu_typ_pred i ->
+          el_rel <∙> nat_glu_exp_pred i ->
+          {{ DG ℕ ∈ glu_univ_elem_core ↘ typ_rel ↘ el_rel }} }
 
   | glu_univ_elem_core_pi :
     `{ forall (in_rel : relation domain)
          IP IEl
-         (OP : forall c c' (equiv_c_c' : {{ Dom c ≈ c' ∈ in_rel }}), typ_pred)
-         (OEl : forall c c' (equiv_c_c' : {{ Dom c ≈ c' ∈ in_rel }}), glu_pred)
+         (OP : forall c (equiv_c_c : {{ Dom c ≈ c ∈ in_rel }}), glu_typ_pred)
+         (OEl : forall c (equiv_c_c : {{ Dom c ≈ c ∈ in_rel }}), glu_exp_pred)
          typ_rel el_rel
          (elem_rel : relation domain),
-          glu_univ_elem_core IP IEl a a' ->
-          per_univ_elem i in_rel a a' ->
-          (forall {c c'} (equiv_c_c' : {{ Dom c ≈ c' ∈ in_rel }}) b b',
+          {{ DG a ∈ glu_univ_elem_core ↘ IP ↘ IEl }} ->
+          {{ DF a ≈ a ∈ per_univ_elem i ↘ in_rel }} ->
+          (forall {c} (equiv_c : {{ Dom c ≈ c ∈ in_rel }}) b,
               {{ ⟦ B ⟧ p ↦ c ↘ b }} ->
-              {{ ⟦ B' ⟧ p' ↦ c' ↘ b' }} ->
-              glu_univ_elem_core (OP _ _ equiv_c_c') (OEl _ _ equiv_c_c') b b') ->
-          per_univ_elem i elem_rel d{{{ Π a p B }}} d{{{ Π a' p' B' }}} ->
-          typ_rel <∙> pi_typ_pred i in_rel IP IEl OP ->
-          el_rel <∙> pi_glu_pred i in_rel IP IEl elem_rel OEl ->
-          glu_univ_elem_core typ_rel el_rel d{{{ Π a p B }}} d{{{ Π a' p' B' }}} }
+              {{ DG b ∈ glu_univ_elem_core ↘ OP _ equiv_c ↘ OEl _ equiv_c }}) ->
+          {{ DF Π a p B ≈ Π a p B ∈ per_univ_elem i ↘ elem_rel }} ->
+          typ_rel <∙> pi_glu_typ_pred i in_rel IP IEl OP ->
+          el_rel <∙> pi_glu_exp_pred i in_rel IP IEl elem_rel OEl ->
+          {{ DG Π a p B ∈ glu_univ_elem_core ↘ typ_rel ↘ el_rel }} }
 
   | glu_univ_elem_core_neut :
     `{ forall typ_rel el_rel,
-          {{ Dom b ≈ b' ∈ per_bot }} ->
-          typ_rel <∙> neut_typ_pred i b ->
-          el_rel <∙> neut_glu_pred i b ->
-          glu_univ_elem_core typ_rel el_rel d{{{ ⇑ a b }}} d{{{ ⇑ a' b' }}} }.
-
+          {{ Dom b ≈ b ∈ per_bot }} ->
+          typ_rel <∙> neut_glu_typ_pred i b ->
+          el_rel <∙> neut_glu_exp_pred i b ->
+          {{ DG ⇑ a b ∈ glu_univ_elem_core ↘ typ_rel ↘ el_rel }} }.
 End Gluing.
 
 #[export]
 Hint Constructors glu_univ_elem_core : mcltt.
 
+Equations glu_univ_elem (i : nat) : glu_typ_pred -> glu_exp_pred -> domain -> Prop by wf i :=
+| i => glu_univ_elem_core i (fun j lt_j_i A Γ M => exists P El, {{ DG A ∈ glu_univ_elem j ↘ P ↘ El }} /\ {{ Γ ⊢ M ® P }}).
 
-Equations glu_univ_elem (i : nat) : typ_pred -> glu_pred -> domain -> domain -> Prop by wf i :=
-| i => glu_univ_elem_core i (fun j lt_j_i A Γ M => exists P El, glu_univ_elem j P El A A /\ P Γ M).
+Definition glu_univ_typ (i : nat) (A : domain) : glu_typ_pred :=
+  fun Γ M => exists P El, {{ DG A ∈ glu_univ_elem i ↘ P ↘ El }} /\ {{ Γ ⊢ M ® P }}.
+Arguments glu_univ_typ i A Γ M/.
 
-
-Definition glu_univ (i : nat) (A : domain) : typ_pred :=
-  fun Γ M => exists P El, glu_univ_elem i P El A A /\ P Γ M.
-Arguments glu_univ i A Γ M/.
-
-Definition univ_glu_pred j i : glu_pred :=
+Definition univ_glu_exp_pred j i : glu_exp_pred :=
     fun Γ m M A =>
       {{ Γ ⊢ m : M }} /\ {{ Γ ⊢ M ≈ Type@j : Type@i }} /\
-        per_univ j A A /\
-        glu_univ j A Γ m.
-Arguments univ_glu_pred j i Γ t T a/.
+        {{ Γ ⊢ m ® glu_univ_typ j A }}.
+Arguments univ_glu_exp_pred j i Γ t T a/.
 
 Section GluingInduction.
-
   Hypothesis
-    (motive : nat -> typ_pred -> glu_pred -> domain -> domain -> Prop)
+    (motive : nat -> glu_typ_pred -> glu_exp_pred -> domain -> Prop)
 
       (case_univ :
-        forall i (j j' : nat)
-          (typ_rel : typ_pred) (el_rel : glu_pred) (lt_j_i : j < i),
-          j = j' ->
-          (forall P El A B, glu_univ_elem j P El A B -> motive j P El A B) ->
-          typ_rel <∙> univ_typ_pred j i ->
-          el_rel <∙> univ_glu_pred j i ->
-          motive i typ_rel el_rel d{{{ 𝕌 @ j }}} d{{{ 𝕌 @ j' }}})
+        forall i (j : nat)
+          (typ_rel : glu_typ_pred) (el_rel : glu_exp_pred) (lt_j_i : j < i),
+          (forall P El A, {{ DG A ∈ glu_univ_elem j ↘ P ↘ El }} -> motive j P El A) ->
+          typ_rel <∙> univ_glu_typ_pred j i ->
+          el_rel <∙> univ_glu_exp_pred j i ->
+          motive i typ_rel el_rel d{{{ 𝕌 @ j }}})
 
       (case_nat :
-        forall i (typ_rel : typ_pred) (el_rel : glu_pred),
-          typ_rel <∙> nat_typ_pred i ->
-          el_rel <∙> nat_glu_pred i ->
-          motive i typ_rel el_rel d{{{ ℕ }}} d{{{ ℕ }}})
+        forall i (typ_rel : glu_typ_pred) (el_rel : glu_exp_pred),
+          typ_rel <∙> nat_glu_typ_pred i ->
+          el_rel <∙> nat_glu_exp_pred i ->
+          motive i typ_rel el_rel d{{{ ℕ }}})
 
       (case_pi :
-        forall i (a a' : domain) (B : typ) (p : env) (B' : typ) (p' : env) (in_rel : relation domain) (IP : typ_pred)
-          (IEl : glu_pred) (OP : forall c c' : domain, {{ Dom c ≈ c' ∈ in_rel }} -> typ_pred)
-          (OEl : forall c c' : domain, {{ Dom c ≈ c' ∈ in_rel }} -> glu_pred) (typ_rel : typ_pred) (el_rel : glu_pred)
+        forall i (a : domain) (B : typ) (p : env) (in_rel : relation domain) (IP : glu_typ_pred)
+          (IEl : glu_exp_pred) (OP : forall c : domain, {{ Dom c ≈ c ∈ in_rel }} -> glu_typ_pred)
+          (OEl : forall c : domain, {{ Dom c ≈ c ∈ in_rel }} -> glu_exp_pred) (typ_rel : glu_typ_pred) (el_rel : glu_exp_pred)
           (elem_rel : relation domain),
-          glu_univ_elem i IP IEl a a' ->
-          motive i IP IEl a a' ->
-          per_univ_elem i in_rel a a' ->
-          (forall (c c' : domain) (equiv_c_c' : {{ Dom c ≈ c' ∈ in_rel }}) (b b' : domain),
+          {{ DG a ∈ glu_univ_elem i ↘ IP ↘ IEl }} ->
+          motive i IP IEl a ->
+          {{ DF a ≈ a ∈ per_univ_elem i ↘ in_rel }} ->
+          (forall (c : domain) (equiv_c : {{ Dom c ≈ c ∈ in_rel }}) (b : domain),
               {{ ⟦ B ⟧ p ↦ c ↘ b }} ->
-              {{ ⟦ B' ⟧ p' ↦ c' ↘ b' }} -> glu_univ_elem i (OP c c' equiv_c_c') (OEl c c' equiv_c_c') b b') ->
-          (forall (c c' : domain) (equiv_c_c' : {{ Dom c ≈ c' ∈ in_rel }}) (b b' : domain),
-              {{ ⟦ B ⟧ p ↦ c ↘ b }} -> {{ ⟦ B' ⟧ p' ↦ c' ↘ b' }} -> motive i (OP c c' equiv_c_c') (OEl c c' equiv_c_c') b b') ->
-          per_univ_elem i elem_rel d{{{ Π a p B }}} d{{{ Π a' p' B' }}} ->
-          typ_rel <∙> pi_typ_pred i in_rel IP IEl OP ->
-          el_rel <∙> pi_glu_pred i in_rel IP IEl elem_rel OEl ->
-          motive i typ_rel el_rel d{{{ Π a p B }}} d{{{ Π a' p' B' }}})
+              {{ DG b ∈ glu_univ_elem i ↘ OP c equiv_c ↘ OEl c equiv_c }}) ->
+          (forall (c : domain) (equiv_c : {{ Dom c ≈ c ∈ in_rel }}) (b : domain),
+              {{ ⟦ B ⟧ p ↦ c ↘ b }} ->
+              motive i (OP c equiv_c) (OEl c equiv_c) b) ->
+          {{ DF Π a p B ≈ Π a p B ∈ per_univ_elem i ↘ elem_rel }} ->
+          typ_rel <∙> pi_glu_typ_pred i in_rel IP IEl OP ->
+          el_rel <∙> pi_glu_exp_pred i in_rel IP IEl elem_rel OEl ->
+          motive i typ_rel el_rel d{{{ Π a p B }}})
 
       (case_neut :
-        forall i (b b' : domain_ne) (a a' : domain)
-          (typ_rel : typ_pred)
-          (el_rel : glu_pred),
-          {{ Dom b ≈ b' ∈ per_bot }} ->
-          typ_rel <∙> neut_typ_pred i b ->
-          el_rel <∙> neut_glu_pred i b ->
-          motive i typ_rel el_rel d{{{ ⇑ a b }}} d{{{ ⇑ a' b' }}})
+        forall i (b : domain_ne) (a : domain)
+          (typ_rel : glu_typ_pred)
+          (el_rel : glu_exp_pred),
+          {{ Dom b ≈ b ∈ per_bot }} ->
+          typ_rel <∙> neut_glu_typ_pred i b ->
+          el_rel <∙> neut_glu_exp_pred i b ->
+          motive i typ_rel el_rel d{{{ ⇑ a b }}})
   .
 
-
   #[local]
-    Ltac def_simp := simp glu_univ_elem in *.
+  Ltac def_simp := simp glu_univ_elem in *.
 
   #[derive(equations=no, eliminator=no), tactic="def_simp"]
-    Equations glu_univ_elem_ind i P El a b
-    (H : glu_univ_elem i P El a b) : motive i P El a b by wf i :=
-  | i, P, El, a, b, H =>
+  Equations glu_univ_elem_ind i P El a
+    (H : glu_univ_elem i P El a) : motive i P El a by wf i :=
+  | i, P, El, a, H =>
       glu_univ_elem_core_ind
         i
-        (fun j lt_j_i A Γ M => glu_univ j A Γ M)
+        (fun j lt_j_i A Γ M => glu_univ_typ j A Γ M)
         (motive i)
-        (fun j j' typ_rel el_rel lt_j_i Heq Htr Hel =>
-           case_univ i j j' typ_rel el_rel lt_j_i
-             Heq
-             (fun P El A B H => glu_univ_elem_ind j P El A B H)
-             Htr
+        (fun j typ_rel el_rel lt_j_i Hty Hel =>
+           case_univ i j typ_rel el_rel lt_j_i
+             (fun P El A H => glu_univ_elem_ind j P El A H)
+             Hty
              Hel)
         (case_nat i)
         _ (* (case_pi i) *)
         (case_neut i)
-        P El a b
+        P El a
         _.
   Next Obligation.
     eapply (case_pi i); def_simp; eauto.
   Qed.
-
 End GluingInduction.
 
-
-Inductive glu_neut i Γ m M c A B : Prop :=
-| glu_neut_make : forall P El,
+Inductive glu_neut i A Γ m M c : Prop :=
+| mk_glu_neut :
     {{ Γ ⊢ m : M }} ->
-    glu_univ_elem i P El A B ->
-    per_bot c c ->
-    (forall Δ σ a, {{ Δ ⊢w σ : Γ }} -> {{ Rne c in length Δ ↘ a }} -> {{ Δ ⊢ m [ σ ] ≈  a : M [ σ ] }}) ->
-    glu_neut i Γ m M c A B.
+    {{ Γ ⊢ M ® glu_univ_typ i A }} ->
+    {{ Dom c ≈ c ∈ per_bot }} ->
+    (forall Δ σ a, {{ Δ ⊢w σ : Γ }} -> {{ Rne c in length Δ ↘ a }} -> {{ Δ ⊢ m[σ] ≈ a : M[σ] }}) ->
+    {{ Γ ⊢ m : M ® c ∈ glu_neut i A }}.
 
-
-Inductive glu_normal i Γ m M a A B : Prop :=
-| glu_normal_make : forall P El,
+Inductive glu_norm i A Γ m M a : Prop :=
+| mk_glu_norm :
     {{ Γ ⊢ m : M }} ->
-    glu_univ_elem i P El A B ->
-    per_top d{{{ ⇓ A a }}} d{{{ ⇓ B a }}} ->
+    {{ Γ ⊢ M ® glu_univ_typ i A }} ->
+    {{ Dom ⇓ A a ≈ ⇓ A a ∈ per_top }} ->
     (forall Δ σ b, {{ Δ ⊢w σ : Γ }} -> {{ Rnf ⇓ A a in length Δ ↘ b }} -> {{ Δ ⊢ m [ σ ] ≈  b : M [ σ ] }}) ->
-    glu_normal i Γ m M a A B.
+    {{ Γ ⊢ m : M ® a ∈ glu_norm i A }}.
 
-
-Inductive glu_typ i Γ M A B : Prop :=
-| glu_typ_make : forall P El,
+Inductive glu_typ i A Γ M : Prop :=
+| mk_glu_typ : forall P El,
     {{ Γ ⊢ M : Type@i }} ->
-    glu_univ_elem i P El A B ->
-    per_top_typ A B ->
-    (forall Δ σ a, {{ Δ ⊢w σ : Γ }} -> {{ Rtyp A in length Δ ↘ a }} -> {{ Δ ⊢ M [ σ ] ≈  a : Type@i }}) ->
-    glu_typ i Γ M A B.
-
+    {{ DG A ∈ glu_univ_elem i ↘ P ↘ El }} ->
+    (forall Δ σ a, {{ Δ ⊢w σ : Γ }} -> {{ Rtyp A in length Δ ↘ a }} -> {{ Δ ⊢ M[σ] ≈ a : Type@i }}) ->
+    {{ Γ ⊢ M ® glu_typ i A }}.
 
 Ltac invert_glu_rel1 :=
   match goal with
-  | H : pi_typ_pred _ _ _ _ _ _ _ |- _ =>
+  | H : pi_glu_typ_pred _ _ _ _ _ _ _ |- _ =>
       progressive_invert H
-  | H : pi_glu_pred _ _ _ _ _ _ _ _ _ _ |- _ =>
+  | H : pi_glu_exp_pred _ _ _ _ _ _ _ _ _ _ |- _ =>
       progressive_invert H
-  | H : neut_typ_pred _ _ _ _ |- _ =>
+  | H : neut_glu_typ_pred _ _ _ _ |- _ =>
       progressive_invert H
-  | H : neut_glu_pred _ _ _ _ _ _ |- _ =>
+  | H : neut_glu_exp_pred _ _ _ _ _ _ |- _ =>
       progressive_invert H
   end.
+
+Variant glu_rel_typ_sub i Δ A σ ρ : Prop :=
+| mk_glu_typ_sub :
+  `{ forall P El,
+        {{ ⟦ A ⟧ ρ ↘ a }} ->
+        {{ DG a ∈ glu_univ_elem i ↘ P ↘ El }} ->
+        {{ Δ ⊢ A[σ] ® P }} ->
+        glu_rel_typ_sub i Δ A σ ρ }.
+
+Definition nil_glu_sub_pred : glu_sub_pred :=
+  fun Δ σ ρ => {{ Δ ⊢s σ : ⋅ }}.
+Arguments nil_glu_sub_pred Δ σ ρ/.
+
+(* The parameters are ordered differently from the Agda version
+   so that we can return "glu_sub_pred". *)
+Variant cons_glu_sub_pred i Γ A (TSb : glu_sub_pred) : glu_sub_pred :=
+| mk_cons_glu_sub_pred :
+  `{ forall P El,
+        {{ Δ ⊢s σ : Γ, A }} ->
+        (* Do we need the following argument?
+           In other words, is it possible to prove that "TSb" respects
+           wf_sub_eq without the following condition? *)
+        {{ Δ ⊢s Wk ∘ σ ≈ Wk∘σ : Γ }} ->
+        {{ ⟦ A ⟧ ρ ↯ ↘ a }} ->
+        {{ DG a ∈ glu_univ_elem i ↘ P ↘ El }} ->
+        {{ Δ ⊢ #0[σ] : A[Wk∘σ] ® ~(ρ 0) ∈ El }} ->
+        {{ Δ ⊢s σ ® ρ ∈ cons_glu_sub_pred i Γ A TSb }} }.
+
+Inductive glu_ctx_env : glu_sub_pred -> ctx -> Prop :=
+| glu_ctx_env_nil :
+  `{ forall Sb,
+        Sb <∙> nil_glu_sub_pred ->
+        {{ EG ⋅ ∈ glu_ctx_env ↘ Sb }} }
+| glu_ctx_env_cons :
+  `{ forall i TSb Sb,
+        {{ EG Γ ∈ glu_ctx_env ↘ TSb }} ->
+        {{ Γ ⊢ A : Type@i }} ->
+        (forall Δ σ ρ,
+            {{ Δ ⊢s σ ® ρ ∈ TSb }} ->
+            glu_rel_typ_sub i Δ A σ ρ) ->
+        Sb <∙> cons_glu_sub_pred i Γ A TSb ->
+        {{ EG Γ, A ∈ glu_ctx_env ↘ Sb }} }.
+
+Variant glu_rel_exp_sub i Δ M A σ ρ : Prop :=
+| mk_glu_exp_sub :
+  `{ forall P El,
+        {{ ⟦ A ⟧ ρ ↘ a }} ->
+        {{ ⟦ M ⟧ ρ ↘ m }} ->
+        {{ DG a ∈ glu_univ_elem i ↘ P ↘ El }} ->
+        {{ Δ ⊢ M[σ] : A[σ] ® m ∈ El }} ->
+        glu_rel_exp_sub i Δ M A σ ρ }.
+
+Variant glu_rel_sub_sub Δ τ (Sb : glu_sub_pred) σ ρ : Prop :=
+| mk_glu_sub_sub :
+  `{ {{ ⟦ τ ⟧s ρ ↘ ρ' }} ->
+     {{ Δ ⊢s τ ∘ σ ® ρ' ∈ Sb }} ->
+     glu_rel_sub_sub Δ τ Sb σ ρ}.
+
+Definition glu_rel_ctx Γ : Prop := exists Sb, {{ EG Γ ∈ glu_ctx_env ↘ Sb }}.
+Arguments glu_rel_ctx Γ/.
+
+Definition glu_rel_exp Γ M A : Prop :=
+  exists Sb,
+    {{ EG Γ ∈ glu_ctx_env ↘ Sb }} /\
+      exists i,
+      forall Δ σ ρ,
+        {{ Δ ⊢s σ ® ρ ∈ Sb }} ->
+        glu_rel_exp_sub i Δ M A σ ρ.
+Arguments glu_rel_exp Γ M A/.
+
+Definition glu_rel_sub Γ τ Γ' : Prop :=
+  exists Sb Sb',
+    {{ EG Γ ∈ glu_ctx_env ↘ Sb }} /\
+    {{ EG Γ' ∈ glu_ctx_env ↘ Sb' }} /\
+      forall Δ σ ρ,
+        {{ Δ ⊢s σ ® ρ ∈ Sb }} ->
+        glu_rel_sub_sub Δ τ Sb' σ ρ.
+Arguments glu_rel_sub Γ τ Γ'/.
+
+Notation "⊩ Γ" := (glu_rel_ctx Γ) (in custom judg at level 80, Γ custom exp).
+Notation "Γ ⊩ M : A" := (glu_rel_exp Γ M A) (in custom judg at level 80, Γ custom exp, M custom exp, A custom exp).
+Notation "Γ ⊩s τ : Γ'" := (glu_rel_sub Γ τ Γ') (in custom judg at level 80, Γ custom exp, τ custom exp, Γ' custom exp).
