theories/Core/Soundness/LogicalRelation/CoreTactics.v
@@ -1,0 +1,14 @@
+From Equations Require Import Equations.
+
+From Mcltt.Core.Soundness Require Import LogicalRelation.Definitions.
+
+Ltac basic_invert_glu_univ_elem H :=
+  progress simp glu_univ_elem in H;
+  inversion H;
+  subst;
+  try rewrite <- glu_univ_elem_equation_1 in *.
+
+Ltac basic_glu_univ_elem_econstructor :=
+  progress simp glu_univ_elem;
+  econstructor;
+  try rewrite <- glu_univ_elem_equation_1 in *.
