theories/Core/Soundness/LogicalRelation/Lemmas.v
@@ -2,19 +2,31 @@ From Coq Require Import Morphisms Morphisms_Relations.
 
 From Mcltt Require Import Base LibTactics.
 From Mcltt.Core Require Import PER Syntactic.Corollaries.
-From Mcltt.Core.Soundness Require Import LogicalRelation.Definitions.
+From Mcltt.Core.Soundness Require Import LogicalRelation.Definitions LogicalRelation.CoreTactics.
 From Mcltt.Core.Soundness Require Export Weakening.Lemmas.
 Import Domain_Notations.
 
+Lemma pi_glu_exp_pred_pi_glu_typ_pred : forall i IR IP IEl (OP : forall c (equiv_c : {{ Dom c ≈ c ∈ IR }}), glu_typ_pred) elem_rel OEl Γ m M a,
+    {{ Γ ⊢ m : M ® a ∈ pi_glu_exp_pred i IR IP IEl elem_rel OEl }} ->
+    (forall Δ m' M' b c (equiv_c : {{ Dom c ≈ c ∈ IR }}),
+        {{ Δ ⊢ m' : M' ® b ∈ OEl _ equiv_c }} ->
+        {{ Δ ⊢ M' ® OP _ equiv_c }}) ->
+    {{ Γ ⊢ M ® pi_glu_typ_pred i IR IP IEl OP }}.
+Proof.
+  inversion_clear 1; econstructor; eauto.
+  intros.
+  edestruct H5 as [? []]; eauto.
+Qed.
+
 Lemma glu_nat_per_nat : forall Γ m a,
     glu_nat Γ m a ->
-    per_nat a a.
+    {{ Dom a ≈ a ∈ per_nat }}.
 Proof.
   induction 1; mauto.
 Qed.
 
 #[local]
- Hint Resolve glu_nat_per_nat : mcltt.
+Hint Resolve glu_nat_per_nat : mcltt.
 
 Lemma glu_nat_escape : forall Γ m a,
     glu_nat Γ m a ->
@@ -26,9 +38,9 @@ Proof.
     | H : _ |- _ => solve [gen_presup H; mauto]
     end.
   assert {{ Γ ⊢w Id : Γ }} by mauto.
-  specialize (H (length Γ)).
-  destruct_conjs.
-  specialize (H0 _ _ _ H2 H3).
+  match_by_head (per_bot c c) ltac:(fun H => specialize (H (length Γ)) as [L []]).
+  clear_dups.
+  assert {{ Γ ⊢ m[Id] ≈ L : ℕ }} by mauto.
   gen_presups.
   mauto.
 Qed.
@@ -49,7 +61,7 @@ Proof.
 Qed.
 
 #[local]
- Hint Resolve glu_nat_resp_equiv : mcltt.
+Hint Resolve glu_nat_resp_equiv : mcltt.
 
 Lemma glu_nat_readback : forall Γ m a,
     glu_nat Γ m a ->
@@ -59,148 +71,152 @@ Lemma glu_nat_readback : forall Γ m a,
       {{ Δ ⊢ m [ σ ] ≈ b : ℕ }}.
 Proof.
   induction 1; intros; progressive_inversion; gen_presups.
-  - transitivity {{{ zero [ σ ] }}}; mauto.
-  - specialize (IHglu_nat _ _ _ H1 H5).
-    transitivity {{{ (succ m') [ σ ]}}}; mauto.
-    transitivity {{{ succ m' [ σ ] }}}; mauto.
+  - transitivity {{{ zero[σ] }}}; mauto.
+  - assert {{ Δ ⊢ m'[σ] ≈ M : ℕ }} by mauto.
+    transitivity {{{ (succ m')[σ] }}}; mauto 3.
+    transitivity {{{ succ m'[σ] }}}; mauto 4.
   - mauto.
 Qed.
 
 #[global]
-  Ltac simpl_glu_rel :=
+Ltac simpl_glu_rel :=
   apply_equiv_left;
   repeat invert_glu_rel1;
   apply_equiv_left;
   destruct_all;
   gen_presups.
 
-
-Lemma glu_univ_elem_univ_lvl : forall i P El A B,
-    glu_univ_elem i P El A B ->
+Lemma glu_univ_elem_univ_lvl : forall i P El A,
+    {{ DG A ∈ glu_univ_elem i ↘ P ↘ El }} ->
     forall Γ T,
-      P Γ T ->
+      {{ Γ ⊢ T ® P }} ->
       {{ Γ ⊢ T : Type@i }}.
 Proof.
+  simpl.
   induction 1 using glu_univ_elem_ind; intros;
     simpl_glu_rel; trivial.
 Qed.
 
-
-Lemma glu_univ_elem_typ_resp_equiv : forall i P El A B,
-    glu_univ_elem i P El A B ->
+Lemma glu_univ_elem_typ_resp_equiv : forall i P El A,
+    {{ DG A ∈ glu_univ_elem i ↘ P ↘ El }} ->
     forall Γ T T',
-      P Γ T ->
+      {{ Γ ⊢ T ® P }} ->
       {{ Γ ⊢ T ≈ T' : Type@i }} ->
-      P Γ T'.
+      {{ Γ ⊢ T' ® P }}.
 Proof.
+  simpl.
   induction 1 using glu_univ_elem_ind; intros;
-    simpl_glu_rel; mauto.
+    simpl_glu_rel; mauto 4.
 
   split; [trivial |].
   intros.
-  specialize (H4 _ _ _ H2 H5); mauto.
+  assert {{ Δ ⊢ T[σ] ≈ V : Type@i }}; mauto.
 Qed.
 
-
-Lemma glu_univ_elem_trm_resp_typ_equiv : forall i P El A B,
-    glu_univ_elem i P El A B ->
+Lemma glu_univ_elem_trm_resp_typ_equiv : forall i P El A,
+    {{ DG A ∈ glu_univ_elem i ↘ P ↘ El }} ->
     forall Γ t T a T',
-      El Γ t T a ->
+      {{ Γ ⊢ t : T ® a ∈ El }} ->
       {{ Γ ⊢ T ≈ T' : Type@i }} ->
-      El Γ t T' a.
+      {{ Γ ⊢ t : T' ® a ∈ El }}.
 Proof.
+  simpl.
   induction 1 using glu_univ_elem_ind; intros;
     simpl_glu_rel; repeat split; mauto.
-  
+
   intros.
-  specialize (H4 _ _ _ H2 H7); mauto.
+  assert {{ Δ ⊢ M[σ] ≈ V : Type@i }}; mauto.
 Qed.
 
-
-Lemma glu_univ_elem_typ_resp_ctx_equiv : forall i P El A B,
-    glu_univ_elem i P El A B ->
+Lemma glu_univ_elem_typ_resp_ctx_equiv : forall i P El A,
+    {{ DG A ∈ glu_univ_elem i ↘ P ↘ El }} ->
     forall Γ T Δ,
-      P Γ T ->
+      {{ Γ ⊢ T ® P }} ->
       {{ ⊢ Γ ≈ Δ }} ->
-      P Δ T.
+      {{ Δ ⊢ T ® P }}.
 Proof.
+  simpl.
   induction 1 using glu_univ_elem_ind; intros;
     simpl_glu_rel; mauto 2;
     econstructor; mauto.
 Qed.
-
 
 Lemma glu_nat_resp_wk' : forall Γ m a,
     glu_nat Γ m a ->
     forall Δ σ,
       {{ Γ ⊢ m : ℕ }} ->
       {{ Δ ⊢w σ : Γ }} ->
-      glu_nat Δ {{{ m [ σ ]}}} a.
+      glu_nat Δ {{{ m[σ] }}} a.
 Proof.
   induction 1; intros; gen_presups.
   - econstructor.
-    transitivity {{{ zero [ σ ]}}}; mauto.
+    transitivity {{{ zero[σ] }}}; mauto.
   - econstructor; [ |mauto].
-    transitivity {{{ (succ m') [σ]}}}; mauto 4.
+    transitivity {{{ (succ m')[σ] }}}; mauto 4.
   - econstructor; trivial.
     intros. gen_presups.
     assert {{ Δ0 ⊢w σ ∘ σ0 : Γ }} by mauto.
-    specialize (H0 _ _ _ H5 H4).
-    transitivity {{{ m [ σ ∘ σ0 ]}}}; mauto 4.
+    assert {{ Δ0 ⊢ m[σ ∘ σ0] ≈ v : ℕ }} by mauto 4.
+    transitivity {{{ m[σ ∘ σ0] }}}; mauto 4.
 Qed.
 
 Lemma glu_nat_resp_wk : forall Γ m a,
     glu_nat Γ m a ->
     forall Δ σ,
       {{ Δ ⊢w σ : Γ }} ->
-      glu_nat Δ {{{ m [ σ ]}}} a.
+      glu_nat Δ {{{ m[σ] }}} a.
 Proof.
   mauto using glu_nat_resp_wk'.
 Qed.
 #[export]
  Hint Resolve glu_nat_resp_wk : mcltt.
 
-Lemma glu_univ_elem_trm_escape : forall i P El A B,
-    glu_univ_elem i P El A B ->
+Lemma glu_univ_elem_trm_escape : forall i P El A,
+    {{ DG A ∈ glu_univ_elem i ↘ P ↘ El }} ->
     forall Γ t T a,
-      El Γ t T a ->
+      {{ Γ ⊢ t : T ® a ∈ El }} ->
       {{ Γ ⊢ t : T }}.
 Proof.
+  simpl.
   induction 1 using glu_univ_elem_ind; intros;
     simpl_glu_rel; mauto 4.
 
-  specialize (H4 (length Γ)).
-  specialize (H (length Γ)).
+  match_by_head (per_bot c c) ltac:(fun H => specialize (H (length Γ)) as [Lc []]).
+  match_by_head (per_bot b b) ltac:(fun H => specialize (H (length Γ)) as [Lb []]).
   assert {{ Γ ⊢w Id : Γ }} by mauto.
-  destruct_all.
-  specialize (H5 _ _ _ _ H6 H9 H7).
-  gen_presup H5.
+  clear_dups.
+  assert {{ Γ ⊢ m[Id] ≈ Lc : M[Id] }} by mauto.
+  gen_presups.
   mauto.
 Qed.
 
-Lemma glu_univ_elem_per : forall i P El A B,
-    glu_univ_elem i P El A B ->
-    exists R, per_univ_elem i R A B.
+Lemma glu_univ_elem_per_univ : forall i P El A,
+    {{ DG A ∈ glu_univ_elem i ↘ P ↘ El }} ->
+    {{ Dom A ≈ A ∈ per_univ i }}.
 Proof.
+  simpl.
   induction 1 using glu_univ_elem_ind; intros; eexists;
     try solve [per_univ_elem_econstructor; try reflexivity; trivial].
 
   - subst. eapply per_univ_elem_core_univ'; trivial.
     reflexivity.
-  - invert_per_univ_elem H3. mauto.
+  - match_by_head per_univ_elem ltac:(fun H => directed invert_per_univ_elem H).
+    mauto.
 Qed.
 
-Lemma glu_univ_elem_trm_per : forall i P El A B,
-    glu_univ_elem i P El A B ->
+Lemma glu_univ_elem_per_elem : forall i P El A,
+    {{ DG A ∈ glu_univ_elem i ↘ P ↘ El }} ->
     forall Γ t T a R,
-      El Γ t T a ->
-      per_univ_elem i R A B ->
-      R a a.
+      {{ Γ ⊢ t : T ® a ∈ El }} ->
+      {{ DF A ≈ A ∈ per_univ_elem i ↘ R }} ->
+      {{ Dom a ≈ a ∈ R }}.
 Proof.
+  simpl.
   induction 1 using glu_univ_elem_ind; intros;
-    try do 2 match_by_head1 per_univ_elem ltac:(fun H => invert_per_univ_elem H);
+    try do 2 match_by_head1 per_univ_elem invert_per_univ_elem;
     simpl_glu_rel;
-    mauto 4.
+    try fold (per_univ j a a);
+    mauto 4 using glu_univ_elem_per_univ.
 
   intros.
   destruct_rel_mod_app.
@@ -211,40 +227,41 @@ Proof.
   econstructor; firstorder eauto.
 Qed.
 
-Lemma glu_univ_elem_trm_typ : forall i P El A B,
-    glu_univ_elem i P El A B ->
+Lemma glu_univ_elem_trm_typ : forall i P El A,
+    {{ DG A ∈ glu_univ_elem i ↘ P ↘ El }} ->
     forall Γ t T a,
-      El Γ t T a ->
-      P Γ T.
+      {{ Γ ⊢ t : T ® a ∈ El }} ->
+      {{ Γ ⊢ T ® P }}.
 Proof.
+  simpl.
   induction 1 using glu_univ_elem_ind; intros;
     simpl_glu_rel;
     mauto 4.
 
   econstructor; eauto.
-  invert_per_univ_elem H3.
+  match_by_head per_univ_elem ltac:(fun H => directed invert_per_univ_elem H).
   intros.
   destruct_rel_mod_eval.
   edestruct H11 as [? []]; eauto.
 Qed.
 
-Lemma glu_univ_elem_trm_univ_lvl : forall i P El A B,
-    glu_univ_elem i P El A B ->
+Lemma glu_univ_elem_trm_univ_lvl : forall i P El A,
+    {{ DG A ∈ glu_univ_elem i ↘ P ↘ El }} ->
     forall Γ t T a,
-      El Γ t T a ->
+      {{ Γ ⊢ t : T ® a ∈ El }} ->
       {{ Γ ⊢ T : Type@i }}.
 Proof.
   intros. eapply glu_univ_elem_univ_lvl; [| eapply glu_univ_elem_trm_typ]; eassumption.
 Qed.
 
-
-Lemma glu_univ_elem_trm_resp_equiv : forall i P El A B,
-    glu_univ_elem i P El A B ->
+Lemma glu_univ_elem_trm_resp_equiv : forall i P El A,
+    {{ DG A ∈ glu_univ_elem i ↘ P ↘ El }} ->
     forall Γ t T a t',
-      El Γ t T a ->
+      {{ Γ ⊢ t : T ® a ∈ El }} ->
       {{ Γ ⊢ t ≈ t' : T }} ->
-      El Γ t' T a.
+      {{ Γ ⊢ t' : T ® a ∈ El }}.
 Proof.
+  simpl.
   induction 1 using glu_univ_elem_ind; intros;
     simpl_glu_rel;
     repeat split; mauto 3.
@@ -256,18 +273,120 @@ Proof.
     invert_per_univ_elem H3.
     intros.
     destruct_rel_mod_eval.
-    assert {{ Δ ⊢ m' : IT [ σ ]}} by eauto using glu_univ_elem_trm_escape.
+    assert {{ Δ ⊢ m' : IT [σ]}} by eauto using glu_univ_elem_trm_escape.
     edestruct H12 as [? []]; eauto.
     eexists; split; eauto.
-    eapply H2; eauto.
+    enough {{ Δ ⊢ m[σ] m' ≈ t'[σ] m' : OT[σ,,m'] }} by eauto.
     assert {{ Γ ⊢ m ≈ t' : Π IT OT }} as Hty by mauto.
-    assert {{ Δ ⊢ IT [ σ ] : Type @ i4 }} by mauto 3.
+    eassert {{ Δ ⊢ IT[σ] : Type@_ }} by mauto 3.
     eapply wf_exp_eq_sub_cong with (Γ := Δ) in Hty; [| eapply sub_eq_refl; mauto 3].
     autorewrite with mcltt in Hty.
     eapply wf_exp_eq_app_cong with (N := m') (N' := m') in Hty; try pi_univ_level_tac; [|mauto 2].
     autorewrite with mcltt in Hty.
     eassumption.
   - intros.
-    assert {{ Δ ⊢ m [ σ ] ≈ t' [ σ ] : M [ σ ] }} by mauto 4.
-    mauto.
+    assert {{ Δ ⊢ m[σ] ≈ t'[σ] : M[σ] }} by mauto 4.
+    mauto 4.
 Qed.
+
+Lemma glu_univ_elem_core_univ' : forall j i typ_rel el_rel,
+    j < i ->
+    (typ_rel <∙> univ_glu_typ_pred j i) ->
+    (el_rel <∙> univ_glu_exp_pred j i) ->
+    {{ DG 𝕌@j ∈ glu_univ_elem i ↘ typ_rel ↘ el_rel }}.
+Proof.
+  intros.
+  unshelve basic_glu_univ_elem_econstructor; mautosolve.
+Qed.
+#[export]
+Hint Resolve glu_univ_elem_core_univ' : mcltt.
+
+Ltac glu_univ_elem_econstructor :=
+  eapply glu_univ_elem_core_univ' + basic_glu_univ_elem_econstructor.
+
+Add Parametric Morphism i : (glu_univ_elem i)
+    with signature glu_typ_pred_equivalence ==> glu_exp_pred_equivalence ==> eq ==> iff as glu_univ_elem_morphism_iff.
+Proof with mautosolve.
+  intros P P' HPP' El El' HElEl'.
+  split; intro Horig; [gen El' P' | gen El P];
+    induction Horig using glu_univ_elem_ind; unshelve glu_univ_elem_econstructor;
+    try (etransitivity; [symmetry + idtac|]; eassumption); eauto.
+Qed.  
+
+Lemma per_univ_elem_pi_clean_inversion : forall i a p B in_rel IP IEl elem_rel typ_rel el_rel,
+  {{ DF a ≈ a ∈ per_univ_elem i ↘ in_rel }} ->
+  {{ DG a ∈ glu_univ_elem i ↘ IP ↘ IEl }} ->
+  {{ DF Π a p B ≈ Π a p B ∈ per_univ_elem i ↘ elem_rel }} ->
+  {{ DG Π a p B ∈ glu_univ_elem i ↘ typ_rel ↘ el_rel }} ->
+  exists (OP : forall c (equiv_c_c : {{ Dom c ≈ c ∈ in_rel }}), glu_typ_pred)
+     (OEl : forall c (equiv_c_c : {{ Dom c ≈ c ∈ in_rel }}), glu_exp_pred),
+      (forall {c} (equiv_c : {{ Dom c ≈ c ∈ in_rel }}) b,
+          {{ ⟦ B ⟧ p ↦ c ↘ b }} ->
+          {{ DG b ∈ glu_univ_elem i ↘ OP _ equiv_c ↘ OEl _ equiv_c }}) /\
+        (typ_rel <∙> pi_glu_typ_pred i in_rel IP IEl OP) /\
+        (el_rel <∙> pi_glu_exp_pred i in_rel IP IEl elem_rel OEl).
+Proof.
+  simpl.
+  pose proof (@relation_equivalence_pointwise domain).
+  intros * Hinper Hinglu Hper Hglu.
+  basic_invert_glu_univ_elem Hglu.
+  handle_per_univ_elem_irrel.
+  do 2 eexists; intuition.
+  - intros Γ A; split; intros.
+    + assert (pi_glu_typ_pred i in_rel0 IP0 IEl0 OP Γ A) as [] by intuition.
+      econstructor; intuition.
+Admitted.
+
+Lemma glu_univ_elem_morphism_per_univ : forall i a a' P El,
+    {{ Dom a ≈ a' ∈ per_univ i }} ->
+    {{ DG a ∈ glu_univ_elem i ↘ P ↘ El }} ->
+    {{ DG a' ∈ glu_univ_elem i ↘ P ↘ El }}.
+Proof.
+  simpl.
+  intros * [elem_rel Hper] Horig. gen P El.
+  induction Hper using per_univ_elem_ind; intros;
+    basic_invert_glu_univ_elem Horig; glu_univ_elem_econstructor; try eassumption; mauto.
+  - handle_per_univ_elem_irrel.
+    etransitivity; [symmetry| ]; eassumption.
+  - handle_per_univ_elem_irrel.
+    intros.
+    (on_all_hyp: destruct_rel_by_assumption in_rel0).
+Admitted.
+
+Lemma per_univ_glu_univ_elem : forall i R a,
+    {{ DF a ≈ a ∈ per_univ_elem i ↘ R }} ->
+    exists P El, {{ DG a ∈ glu_univ_elem i ↘ P ↘ El }}.
+Proof.
+  simpl.
+  induction 1 using per_univ_elem_ind; intros;
+    try solve [do 2 eexists; unshelve (glu_univ_elem_econstructor; try reflexivity; subst; trivial)].
+
+  - destruct IHper_univ_elem as [? []].
+    do 2 eexists.
+    glu_univ_elem_econstructor; try reflexivity; mauto.
+    + etransitivity; [symmetry |]; eassumption.
+    + instantiate (1 := fun (c : domain) (equiv_c : in_rel c c) Γ M A m =>
+                          forall b P El,
+                            {{ ⟦ B' ⟧ p' ↦ c ↘ b }} ->
+                            glu_univ_elem i P El b ->
+                            {{ Γ ⊢ M : A ® m ∈ El }}).
+      instantiate (1 := fun (c : domain) (equiv_c : in_rel c c) Γ A =>
+                          forall b P El,
+                            {{ ⟦ B' ⟧ p' ↦ c ↘ b }} ->
+                            glu_univ_elem i P El b ->
+                            {{ Γ ⊢ A ® P }}).
+      intros.
+      (on_all_hyp: destruct_rel_by_assumption in_rel).
+      functional_eval_rewrite_clear.
+      rewrite glu_univ_elem_morphism_iff; try (eassumption + reflexivity);
+        split; intros; intuition.
+      * admit.
+      * admit.
+    + enough {{ DF Π A p B ≈ Π A' p' B' ∈ per_univ_elem i ↘ elem_rel }} by (etransitivity; [symmetry |]; eassumption).
+      per_univ_elem_econstructor; mauto.
+      intros.
+      (on_all_hyp: destruct_rel_by_assumption in_rel).
+      mauto.
+  - do 2 eexists.
+    basic_glu_univ_elem_econstructor; try reflexivity; mauto.
+Admitted.
