theories/Core/Syntactic/System/Lemmas.v
@@ -87,19 +87,6 @@ Proof with mautosolve.
   assert (m <= max n m) by lia...
 Qed.
 
-#[global]
-  Ltac pi_univ_level_tac :=
-  match goal with
-  | |- {{ ~_ ⊢s ~_ : ~_ }} => mauto 4
-  | H : {{ ~?Δ ⊢ ~?A : ~(a_typ ?j) }} |- {{ ~?Δ , ~?A ⊢ ~?B : ~(a_typ ?i) }} =>
-      eapply lift_exp_max_right; mauto 4
-  | |- {{ ~?Δ ⊢ ~?A : ~(a_typ ?j) }} =>
-      eapply lift_exp_max_left; mauto 4
-  end.
-
-#[export]
-  Hint Rewrite -> wf_exp_eq_pi_sub using pi_univ_level_tac : mcltt.
-
 Lemma lift_exp_eq_ge : forall {Γ A A' n m}, n <= m -> {{ Γ ⊢ A ≈ A': Type@n }} -> {{ Γ ⊢ A ≈ A' : Type@m }}.
 Proof with mautosolve.
   induction 1; subst...
