theories/Core/Syntactic/System/Tactics.v
@@ -1,6 +1,19 @@
 From Mcltt Require Import Base LibTactics.
-From Mcltt Require Export System.Definitions.
+From Mcltt Require Export System.Definitions System.Lemmas.
 Import Syntax_Notations.
+
+#[global]
+Ltac pi_univ_level_tac :=
+  match goal with
+  | |- {{ ~_ ⊢s ~_ : ~_ }} => mauto 4
+  | H : {{ ~?Δ ⊢ ~?A : Type@?j }} |- {{ ~?Δ , ~?A ⊢ ~?B : Type@?i }} =>
+      eapply lift_exp_max_right; mauto 4
+  | |- {{ ~?Δ ⊢ ~?A : Type@?j }} =>
+      eapply lift_exp_max_left; mauto 4
+  end.
+
+#[export]
+Hint Rewrite -> wf_exp_eq_pi_sub using pi_univ_level_tac : mcltt.
 
 #[local]
 Ltac invert_wf_ctx1 H :=
